MESI: started proving [InvExcl]; the last invariant

src/Ex/Mesi/MesiInvExcl.v
@@ -34,6 +34,106 @@ Definition InvExcl (st: MState): Prop :=
     eost <+- (bst_oss st)@[eidx];
       InvObjExcl0 eidx eost (bst_oss st) (bst_msgs st).
 
+Section Facts.
+
+  (** [ObjExcl0] *)
+
+  Lemma ObjExcl0_enqMP_inv:
+    forall oidx ost msgs midx msg,
+      ObjExcl0 oidx ost (enqMP midx msg msgs) ->
+      ObjExcl0 oidx ost msgs.
+  Proof.
+    unfold ObjExcl0; intros.
+    dest; split; [assumption|].
+    disc_MsgsP H0; assumption.
+  Qed.
+
+  Lemma ObjExcl0_enqMsgs_inv:
+    forall oidx ost msgs nmsgs,
+      ObjExcl0 oidx ost (enqMsgs nmsgs msgs) ->
+      ObjExcl0 oidx ost msgs.
+  Proof.
+    unfold ObjExcl0; intros.
+    dest; split; [assumption|].
+    disc_MsgsP H0; assumption.
+  Qed.
+
+  Lemma ObjExcl0_other_midx_deqMP_inv:
+    forall oidx ost msgs midx,
+      ObjExcl0 oidx ost (deqMP midx msgs) ->
+      midx <> downTo oidx ->
+      ObjExcl0 oidx ost msgs.
+  Proof.
+    unfold ObjExcl0; intros.
+    dest; split; [assumption|].
+    disc_MsgsP H1; assumption.
+  Qed.
+
+  Lemma ObjExcl0_other_midx_deqMsgs_inv:
+    forall oidx ost msgs (rmsgs: list (Id Msg)),
+      ObjExcl0 oidx ost (deqMsgs (idsOf rmsgs) msgs) ->
+      NoDup (idsOf rmsgs) ->
+      Forall (FirstMPI msgs) rmsgs ->
+      Forall (fun midx => midx <> downTo oidx) (idsOf rmsgs) ->
+      ObjExcl0 oidx ost msgs.
+  Proof.
+    unfold ObjExcl0; intros.
+    dest; split; [assumption|].
+    apply MsgsP_other_midx_deqMsgs_inv in H3.
+    - assumption.
+    - simpl.
+      simpl; apply (DisjList_spec_1 idx_dec); intros.
+      rewrite Forall_forall in H2; specialize (H2 _ H4).
+      intro Hx; dest_in; auto.
+  Qed.
+
+  Lemma ObjExcl0_other_msg_id_deqMP_inv:
+    forall oidx ost msgs midx,
+      ObjExcl0 oidx ost (deqMP midx msgs) ->
+      forall msg,
+        FirstMP msgs midx msg ->
+        msg.(msg_id) <> mesiInvRs ->
+        ObjExcl0 oidx ost msgs.
+  Proof.
+    unfold ObjExcl0; intros.
+    dest; split; [assumption|].
+    eapply MsgsP_other_msg_id_deqMP_inv in H2;
+      [|eassumption|simpl; intuition].
+    assumption.
+  Qed.
+
+  Lemma ObjExcl0_other_msg_id_deqMsgs_inv:
+    forall oidx ost msgs rmsgs,
+      ObjExcl0 oidx ost (deqMsgs (idsOf rmsgs) msgs) ->
+      NoDup (idsOf rmsgs) ->
+      Forall (FirstMPI msgs) rmsgs ->
+      Forall (fun idm => (valOf idm).(msg_id) <> mesiInvRs) rmsgs ->
+      ObjExcl0 oidx ost msgs.
+  Proof.
+    unfold ObjExcl0; intros.
+    dest; split; [assumption|].
+    eapply MsgsP_other_msg_id_deqMsgs_inv in H3; try assumption.
+    simpl; apply (DisjList_spec_1 idx_dec); intros.
+    apply in_map_iff in H4; dest; subst.
+    rewrite Forall_forall in H2; specialize (H2 _ H5).
+    intro Hx; dest_in; auto.
+  Qed.
+
+  Ltac disc_ObjExcl0_msgs H :=
+    repeat
+      (first [apply ObjExcl0_enqMP_inv in H
+             |apply ObjExcl0_enqMsgs_inv in H
+             |apply ObjExcl0_other_midx_deqMP_inv in H; [|solve_chn_neq]
+             |apply ObjExcl0_other_midx_deqMsgs_inv in H;
+              [|eassumption|eassumption|] (** FIXME: need to debug when not working *)
+             |eapply ObjExcl0_other_msg_id_deqMP_inv in H;
+              [|eassumption|congruence]
+             |eapply ObjExcl0_other_msg_id_deqMsgs_inv in H;
+              [|eassumption|eassumption|] (** FIXME: need to debug when not working *)
+      ]).
+
+End Facts.
+
 Section InvExcl.
   Variable (tr: tree).
   Hypothesis (Htr: tr <> Node nil).
@@ -134,6 +234,14 @@ Section InvExcl.
       + apply tree2Topo_minds_merqs_disj.
   Qed.
 
+  Corollary mesi_InvExcl_InvTrsIns: InvTrsIns impl InvExcl.
+  Proof.
+    red; intros.
+    inv H1.
+    eapply mesi_InvExcl_ext_in; eauto.
+    apply (mesi_InObjInds H).
+  Qed.
+
   Lemma mesi_InvExcl_ext_out:
     forall oss orqs msgs,
       InvExcl {| bst_oss := oss; bst_orqs := orqs; bst_msgs := msgs |} ->
@@ -191,12 +299,162 @@ Section InvExcl.
           rewrite Heost in H0; simpl in H0.
           eassumption.
       + apply tree2Topo_minds_merss_disj.
-  Qed.      
+  Qed.
 
-  Lemma mesi_InvExcl_step:
-    Invariant.InvStep impl step_m InvExcl.
+  Corollary mesi_InvExcl_InvTrsOuts: InvTrsOuts impl InvExcl.
+  Proof.
+    red; intros.
+    inv H1.
+    eapply mesi_InvExcl_ext_out; eauto.
+    apply (mesi_InObjInds H).
+  Qed.
+
+  Definition InvExclMsgOutPred: MsgOutPred :=
+    fun eout oss orqs =>
+      caseDec sig_dec (sigOf eout) True
+              (List.concat
+                 (map (fun oidx =>
+                         [((rqUpFrom (l1ExtOf oidx), (MRq, Spec.getRq)), False);
+                            ((rqUpFrom (l1ExtOf oidx), (MRq, Spec.setRq)), False)])
+                      (c_l1_indices cifc))).
+
+  Lemma InvExclMsgOutPred_good:
+    GoodMsgOutPred topo InvExclMsgOutPred.
   Proof.
   Admitted.
+
+  Lemma mesi_InvExcl_InvTrs_init:
+    forall st1,
+      Reachable (steps step_m) impl st1 ->
+      InvExcl st1 ->
+      forall oidx ridx ins outs st2,
+        SubList (idsOf ins) (sys_merqs impl) ->
+        step_m impl st1 (RlblInt oidx ridx ins outs) st2 ->
+        AtomicInv
+          InvExclMsgOutPred
+          ins st1 [RlblInt oidx ridx ins outs] outs st2 /\
+        InvExcl st2.
+  Proof.
+  Admitted.
+
+  Ltac disc_rule_custom ::=
+    try disc_AtomicInv.
+
+  Lemma mesi_InvExcl_InvTrs: InvTrs impl InvExcl.
+  Proof.
+    eapply inv_atomic_InvTrs;
+      [red; intros; eapply mesi_InvExcl_InvTrsIns; eauto
+      |red; intros; eapply mesi_InvExcl_InvTrsOuts; eauto
+      |].
+    instantiate (1:= AtomicInv InvExclMsgOutPred).
+
+    red; intros.
+    destruct H1.
+    generalize dependent ist2.
+    induction H3; simpl; intros; subst;
+      [inv_steps; apply mesi_InvExcl_InvTrs_init; auto|].
+
+    inv_steps.
+    pose proof (reachable_steps H H9) as Hr1.
+    pose proof (reachable_steps Hr1 (steps_singleton H11)) as Hr2.
+
+    pose proof (tree2Topo_TreeTopoNode tr 0) as Htn.
+    (* pose proof (footprints_ok *)
+    (*               msiSv_impl_ORqsInit *)
+    (*               msiSv_impl_GoodRqRsSys Hr1) as Hftinv. *)
+    (* pose proof (upLockInv_ok *)
+    (*               msiSv_impl_ORqsInit *)
+    (*               msiSv_impl_GoodRqRsSys *)
+    (*               msiSv_impl_RqRsDTree Hr1) as Hpulinv. *)
+
+    specialize (IHAtomic H1 _ H9); dest.
+    inv_step.
+
+    simpl in H13; destruct H13; [subst|apply in_app_or in H7; destruct H7].
+    
+    - (*! Cases for the main memory *)
+
+      (** Abstract the root. *)
+      assert (In (rootOf (fst (tree2Topo tr 0)))
+                 (c_li_indices (snd (tree2Topo tr 0)))) as Hin.
+      { rewrite c_li_indices_head_rootOf by assumption.
+        left; reflexivity.
+      }
+
+      remember (rootOf (fst (tree2Topo tr 0))) as oidx; clear Heqoidx.
+
+      (** Do case analysis per a rule. *)
+      apply in_app_or in H14; destruct H14.
+
+      1: { (** Rules per a child *)
+        apply concat_In in H7; destruct H7 as [crls [? ?]].
+        apply in_map_iff in H7; destruct H7 as [cidx [? ?]]; subst.
+
+        (** Derive that the child has the parent. *)
+        assert (parentIdxOf (fst (tree2Topo tr 0)) cidx = Some oidx)
+          by (apply subtreeChildrenIndsOf_parentIdxOf; auto).
+
+        dest_in.
+        all: admit.
+      }
+
+      dest_in.
+      all: admit.
+
+    - (*! Cases for Li caches *)
+      apply in_map_iff in H7; destruct H7 as [oidx [? ?]]; subst; simpl in *.
+
+      pose proof (c_li_indices_tail_has_parent Htr _ _ H8).
+      destruct H7 as [pidx [? ?]].
+      pose proof (Htn _ _ H10); dest.
+
+      (** Do case analysis per a rule. *)
+      apply in_app_or in H14; destruct H14.
+
+      1: { (** Rules per a child *)
+        apply concat_In in H14; destruct H14 as [crls [? ?]].
+        apply in_map_iff in H14; destruct H14 as [cidx [? ?]]; subst.
+
+        (** Derive that the child has the parent. *)
+        assert (parentIdxOf (fst (tree2Topo tr 0)) cidx = Some oidx)
+          by (apply subtreeChildrenIndsOf_parentIdxOf; auto).
+
+        dest_in.
+        all: admit.
+      }
+
+      dest_in.
+      all: admit.
+
+    - (*! Cases for L1 caches *)
+      apply in_map_iff in H7; destruct H7 as [oidx [? ?]]; subst.
+
+      pose proof (c_l1_indices_has_parent Htr _ _ H8).
+      destruct H7 as [pidx [? ?]].
+      pose proof (Htn _ _ H10); dest.
+
+      (** Discharge an invariant that holds only for L1 caches. *)
+      (* red in Hl1d; simpl in Hl1d. *)
+      (* rewrite Forall_forall in Hl1d; specialize (Hl1d _ H2). *)
+      (* simpl in H5; rewrite H5 in Hl1d; simpl in Hl1d. *)
+
+      (** Do case analysis per a rule. *)
+      dest_in.
+      all: admit.
+
+  Qed.
+
+  Lemma mesi_InvExcl_step:
+    InvStep impl step_m InvExcl.
+  Proof.
+    apply invSeq_serializable_invStep.
+    - apply mesi_InvExcl_init.
+    - apply inv_trs_seqSteps.
+      apply mesi_InvExcl_InvTrs.
+    - eapply rqrs_Serializable.
+      + apply mesi_GoodORqsInit.
+      + apply mesi_RqRsSys.
+  Qed.
 
   Lemma mesi_InvExcl_ok:
     Invariant.InvReachable impl step_m InvExcl.
